\documentclass[12pt]{article}
\usepackage[utf8]{inputenc}
\usepackage{amsmath, amsfonts, amssymb}
\usepackage[a4paper, margin=1in]{geometry}
\usepackage{varwidth}

\title{Random Variables and Stochastic Process (AI5030)}
\author{Soumyajit Chatterjee\\AI22MTECH02005 }


\begin{document}

\maketitle

\section*{Question 56 (2019)}
There are two sets of observations on a random vector $(X,Y)$. Consider a simple linear regression model with an intercept for regressing $Y$ on $X$. Let $\hat{\beta_i}$ be the least square estimate of the regression coefficient obtained from the ith (i=1, 2) set consisting of $n_i$ observations $(n_1, n_2) > 2$. Let $\hat{\beta_0}$ be the least square  estimate obtained from the pooled sample size $n_1+n_2$. If it is known that $\hat{\beta_1} > \hat{\beta_2} > 0$, which of the following statements is true ?
\vspace{1cm}

1. $\hat{\beta_2} < \hat{\beta_0} < \hat{\beta_1}$

2. $\hat{\beta_0}$ \text{ may lie outside } $(\hat{\beta_2}, \hat{\beta_1})$ but cannot exceed $\hat{\beta_1} + \hat{\beta_2}$

3. $\hat{\beta_0}$ \text{ may lie outside } $(\hat{\beta_2}, \hat{\beta_1})$ but cannot be negative

4. $\hat{\beta_0}$ can be negative
\vspace{1cm}

\section*{Solution}

\subsection*{Derivation of Least Square estimator}

Let a straight line be estimated on a vector $(X,Y)$ using an estimator such that:
\begin{equation}
\hat{Y} = \hat{\beta} X
\end{equation}

\noindent The error in approximation with respect to the actual distribution can be then given as,

\begin{equation}
E = \sum (\hat{Y} -Y)^2
\end{equation}

\noindent The above equation can be re-written in the matrix form as:

\begin{align}
E &= (\hat{Y} - Y)^T (\hat{Y} - Y)\\
&= \hat{Y}^T\hat{Y} - Y^T\hat{Y} - \hat{Y}^TY + Y^TY
\end{align}

\noindent We know that $\hat{Y} = \hat{\beta} X$, therefore substituting in equation 4:

\begin{equation}
E = Y^TY - 2\hat{\beta}^TX^TY + \hat{\beta}^TX^TX\hat{\beta}
\end{equation}

\vspace{2mm}

\noindent Differentiating the above equation w.r.t $\hat{\beta}$ and equating it to 0 to obtain the $\hat{\beta}$ that minimizes the error.

\begin{equation}
\dfrac{dE}{d\hat{\beta}} = -2X^TY + 2X^TX\hat{\beta} = 0
\end{equation}

\begin{equation}
X^TX\hat{\beta} = X^TY
\end{equation}

\begin{equation}
\hat{\beta} = (X^TX)^{-1}X^TY
\end{equation}

\vspace{3mm}
\noindent We know that the term $X^TX$ is the term $\sum X^2$ which is always positive. Therefore, the term that determines the sign of $\hat{\beta}$ is $X^TY$

\vspace{3mm}
\noindent We now take two cases which eliminates our options:

\vspace{3mm}
\noindent \textbf{Case 1:}
\vspace{3mm}

\noindent Sample $n_1$,
\vspace{3mm}

\begin{center}

X = $
\begin{bmatrix}
1\\2\\3
\end{bmatrix}
$
\hspace{2mm} Y = $
\begin{bmatrix}
-2\\-4\\-6
\end{bmatrix}
$
\hspace{2mm} $\hat{\beta_1} =  -2$
\end{center}

\vspace{3mm}

\noindent Sample $n_2$,
\vspace{3mm}

\begin{center}

X = $
\begin{bmatrix}
4\\5\\6
\end{bmatrix}
$
\hspace{2mm} Y = $
\begin{bmatrix}
-8\\-10\\-12
\end{bmatrix}
$
\hspace{2mm} $\hat{\beta_2} =  -2$
\end{center}

\vspace{3mm}

\noindent Sample $n_1+n_2$,
\vspace{3mm}

\begin{center}

X = $
\begin{bmatrix}
1\\2\\3\\4\\5\\6
\end{bmatrix}
$
\hspace{2mm} Y = $
\begin{bmatrix}
-2\\-4\\-6\\-8\\-10\\-12
\end{bmatrix}
$
\hspace{2mm} $\hat{\beta_0} =  -2$
\end{center}

\vspace{3mm}

\noindent For the above case, $\hat{\beta_0}$ is negative and $\hat{\beta_1} = \hat{\beta_2} = \hat{\beta_0}$, therefore, the options (1) and (3) are invalid.

\clearpage

\vspace{3mm}
\noindent \textbf{Case 2:}
\vspace{3mm}

\noindent Sample $n_1$,
\vspace{3mm}

\begin{center}

X = $
\begin{bmatrix}
1\\2\\3
\end{bmatrix}
$
\hspace{2mm} Y = $
\begin{bmatrix}
-2\\-4\\-6
\end{bmatrix}
$
\hspace{2mm} $\hat{\beta_1} =  -2$
\end{center}

\vspace{3mm}

\noindent Sample $n_2$,
\vspace{3mm}

\begin{center}

X = $
\begin{bmatrix}
4\\5\\6
\end{bmatrix}
$
\hspace{2mm} Y = $
\begin{bmatrix}
12\\15\\18
\end{bmatrix}
$
\hspace{2mm} $\hat{\beta_2} =  3$
\end{center}

\vspace{3mm}

\noindent Sample $n_1+n_2$,
\vspace{3mm}

\begin{center}

X = $
\begin{bmatrix}
1\\2\\3\\4\\5\\6
\end{bmatrix}
$
\hspace{2mm} Y = $
\begin{bmatrix}
-2\\-4\\-6\\12\\15\\18
\end{bmatrix}
$
\hspace{2mm} $\hat{\beta_0} =  5$
\end{center}

\vspace{3mm}

\noindent Here, $\hat{\beta_1}$ is -2 and $\hat{\beta_2}$ is 3. Now, $\hat{\beta_1} + \hat{\beta_2} = -2+3=1$. But we see that $\hat{\beta_0} = 5$ which is outside the range of $\hat{\beta_1} + \hat{\beta_2}$

\vspace{3mm}
\noindent Therefore, option (2) is also incorrect. The only option which remains i.e option (4) is correct.

\end{document}
